# our own namespaces for properties, classes, and shacl shapes:
@prefix pxp: <https://w3id.org/zpid/ontology/properties/> .
@prefix pxc: <https://w3id.org/zpid/ontology/classes/> .
@prefix pxs: <https://w3id.org/zpid/shapes/> .

# important namespaces we reuse because ancestors of our own classes and properties are from there (superclasses and superproperties are from these namespaces):
@prefix bf: <http://id.loc.gov/ontologies/bibframe/> .
@prefix bflc: <http://id.loc.gov/ontologies/bflc/> .
@prefix skos: <http://www.w3.org/2004/02/skos/core#> .
@prefix schema: <https://schema.org/> .

# mainly used for mapping of properties and classes to other ontologies:
@prefix dblp: <https://dblp.org/rdf/schema#> .
@prefix bibo: <http://purl.org/ontology/bibo/>.

# basic ontology namespaces:
@prefix rdf: <http://www.w3.org/1999/02/22-rdf-syntax-ns#> .
@prefix rdfs: <http://www.w3.org/2000/01/rdf-schema#> .
@prefix owl: <http://www.w3.org/2002/07/owl#> .
@prefix xml: <http://www.w3.org/XML/1998/namespace> .
@prefix dct:  <http://purl.org/dc/terms/> .
@prefix xsd: <http://www.w3.org/2001/XMLSchema#> .
@prefix vann: <http://purl.org/vocab/vann/> .

<https://w3id.org/zpid/ontology/properties>
   rdf:type owl:Ontology ; #voaf:Vocabulary ;
   vann:preferredNamespacePrefix "pxp" ;
   vann:preferredNamespaceUri "https://w3id.org/zpid/ontology/properties/" ;
   dct:title "ZPID/PSYNDEX properties" ;
   #dct:license <...> ;
   dct:description "New properties that we need to define because there aren't any in BIBFRAME and related we can reuse"@en ;
   dct:issued "2022-07-01" ;
   dct:modified "2022-11-28"^^xsd:date ;
   skos:historyNote "See the commit history for this vocabulary at https://github.com/." ;
   #dct:publisher <...> ;
   #dct:creator <...> ;
.
<https://w3id.org/zpid/ontology/classes>
   rdf:type owl:Ontology ; #voaf:Vocabulary ;
   vann:preferredNamespacePrefix "pxc" ;
   vann:preferredNamespaceUri "https://w3id.org/zpid/ontology/classes/" ;
   dct:title "ZPID/PSYNDEX classes" ;
   #dct:license <...> ;
   dct:description "New classes that we need to define because there aren't any in BIBFRAME and related we can reuse"@en ;
   dct:issued "2022-07-01" ;
   dct:modified "2022-11-28"^^xsd:date ;
   skos:historyNote "See the commit history for this vocabulary at https://github.com/." .
pxc:DFK a owl:Class;
    rdfs:subClassOf bf:Local;
    rdfs:label "DFK"@de, "DFK"@en;
    rdfs:comment "The DFK is the unique identifier of a publication in PSYNDEX. It is a string of 8 numbers."@en;
pxc:PsychAuthorsID a owl:Class;
    rdfs:subClassOf bf:Local;
    rdfs:label "PsychAuthors-Kennung"@de, "PsychAuthors ID"@en;
    rdfs:comment "The PsychAuthors ID is the unique identifier of a person in our legacy psychauthors authority file of psychologists."@en;
pxc:TranslatedTitle a owl:Class;
    rdfs:subClassOf bf:VariantTitle;
    rdfs:label "Original title translated into English or German"@en;
rdfs:description "Title as translated either by the creator, by a ZPID cataloger/indexer or some automated translation service like Deepl. Usually contains subtitle as well; Language is en if original work language is de; if work language is en, the translated title has language en." .
pxc:Abstract a owl:Class;
    rdfs:subClassOf bf:Summary;
    rdfs:label "Abstract"@en, "Abstract"@de;
.
pxc:PlainLanguageSummary a owl:Class;
    rdfs:subClassOf bf:Summary;
    rdfs:label "Plain Language Summary"@en, "Laienzusammenfassung"@de;
.
pxc:WeightedTopic a owl:Class;
    rdfs:subClassOf bf:Topic;
    rdfs:label "Weighted Topic"@en, "Gewichtetes Schlagwort"@de;
    rdfs:comment "A topic that has more weight than others. One that is most essential in describing the work and what it is about."@en;
.
pxc:SubjectHeading a owl:Class;
    rdfs:subClassOf bf:Classification;
    rdfs:label "Psychological Subject Heading Classification"@en, "Psychologische Inhaltsklassifikation"@de;
.
pxc:ControlledMethod a owl:Class;
    rdfs:subClassOf bf:Classification;
    rdfs:label "Controlled Method Classification"@en, "Klassifikation der kontrollierten Methode"@de;
    rdfs:comment "The scientific study methodology used to create the study described within the work."@en;
.
pxc:AgeGroup a owl:Class;
    rdfs:subClassOf bflc:DemographicGroup;
    rdfs:label "Age Group of study population or of instrument target group"@en, "Altersbereich der Studienpopulation oder der Testzielgruppe"@de; 
.
pxc:PopulationLocation a owl:Class;
    rdfs:subClassOf bf:GeographicCoverage;
    rdfs:label "Population Location"@en, "Ort der Studienpopulation"@de; 
.
pxp:contributionPosition
  a rdf:Property ;
  rdfs:label "contributor position"@en ;
  rdfs:comment "Position of contributor (within the creator sequence) of the publication, starting with 1. for first author or contributor"@en ;
  rdfs:domain bf:Contribution ;
  rdfs:range xsd:integer;
  owl:equivalentProperty dblp:signatureOrdinal, <http://www.wikidata.org/entity/P478>; rdfs:subPropertyOf schema:position, bf:qualifier
.
pxp:inIssue a rdf:Property;
  rdfs:label "published in journal issue"@en ;
  rdfs:comment "The issue of the journal in which the publication was published."@en ;
    rdfs:subPropertyOf bf:part, bibo:locator; # bf:part is equivalent to MARC subfield $g eg in field 773; a literal that contains volume, issue and page range of a "hosted item" - which is an article in a journal.
    owl:equivalentProperty dblp:publishedInJournalVolumeIssue, <http://purl.org/ontology/bibo/issue>, <http://prismstandard.org/namespaces/basic/2.0/issueIdentifier>, schema:issueNumber, <http://www.wikidata.org/entity/P433>;
    rdfs:domain bflc:Relationship;
    rdfs:range xsd:string;
.
pxp:inVolume a rdf:Property;
  rdfs:label "published in journal volume"@en ;
  rdfs:comment "The volume of the journal in which the publication was published."@en ;
    rdfs:subPropertyOf bf:part, bibo:locator; 
    owl:equivalentProperty dblp:publishedInJournalVolumeIssue, <http://www.wikidata.org/entity/P478>, <http://prismstandard.org/namespaces/basic/2.0/volume>, schema:volumeNumber;
    rdfs:domain bflc:Relationship;
    rdfs:range xsd:string;
.
pxp:pageStart a rdf:Property;
    rdfs:label "first page"@en, "erste Seite"@de;
    rdfs:comment "The page within a journal issue or a book on which an article or chapter begins; the first page of the part."@en;
    rdfs:subPropertyOf bf:part, bibo:locator;
    owl:equivalentProperty schema:pageStart, <http://prismstandard.org/namespaces/1.2/basic/startingPage>, bibo:pageStart;
    rdfs:domain bflc:Relationship;
    rdfs:range xsd:integer;
.
pxp:pageEnd a rdf:Property;
    rdfs:label "last page"@en, "letzte Seite"@de;
    rdfs:comment "The page within a journal issue or a book on which an article or chapter ends; the last page of the part."@en;
    rdfs:subPropertyOf bf:part, bibo:locator;
    owl:equivalentProperty schema:pageEnd, <http://prismstandard.org/namespaces/1.2/basic/endingPage>, bibo:pageEnd;
    rdfs:domain bflc:Relationship;
    rdfs:range xsd:integer;
.
pxc:ArticleNumber a owl:Class;
    rdfs:label "Article number"@en, "Artikelnummer"@de;
    rdfs:comment "Alphanumerica identifier of a journal article within that journal. Usually for electronic journal articles where no start or end page is given. Value (the number/identifier) is found in a rdf:value property, as is usual for bf:Identifier subclasses.";
    rdfs:subClassOf bf:Identifier;
    .
pxp:PageCount a owl:Class;
    rdfs:subClassOf bf:Extent;
 #owl:equivalentProperty <http://purl.org/spar/fabio/hasPageCount>.
.
pxp:issuanceType a rdf:Property;
    rdfs:label "Erscheinungsform"@de, "Issuance Type"@en;
    skos:altLabel "Publication type"@en, "Publikationstyp"@de;
    rdfs:comment "Describes the type of publication an instance was issued as, including its bibliographic level (former BE field in PSYNDEX) = whether it is a standalone thing or a dependent component part. Examples: Journal Article, Edited Book"@en;
    rdfs:domain bf:Instance;
    rdfs:range skos:Concept;
    . 
pxp:mediaCarrier a rdf:Property;
    rdfs:label "Medien-/Datentr√§gertyp"@de, "Media and Carrier Type"@en;
    rdfs:comment "Describes an instance's combined medium and carrier type. Close approximation of former field MT and MT2 in PSYNDEX"@en;
    rdfs:domain bf:Instance;
    rdfs:range skos:Concept;
. 
